coq/LLVMGen/Correctness_Alloc.v
@@ -38,13 +38,13 @@ Proof.
 Admitted.
 
 Lemma no_dshptr_aliasing_cons :
-  forall (memH : memoryH) (σ : evalContext) (size : Int64.int),
-    no_dshptr_aliasing (DSHPtrVal (memory_next_key memH) size :: σ) ->
+  forall (memH : memoryH) (σ : evalContext) (size : Int64.int) b,
+    no_dshptr_aliasing ((DSHPtrVal (memory_next_key memH) size , b):: σ) ->
     no_dshptr_aliasing σ.
 Proof.
   intros * st_no_dshptr_aliasing. repeat intro.
   specialize (st_no_dshptr_aliasing (S n) (S n')). cbn in *.
-  specialize (st_no_dshptr_aliasing _ _ _ H H0).
+  specialize (st_no_dshptr_aliasing _ _ _ _ _ H H0).
   inversion st_no_dshptr_aliasing. subst. reflexivity.
 Qed.
 
@@ -333,7 +333,7 @@ Proof.
     - cbn. intros. rewrite context_l0 in mem_is_inv.
       cbn in *. specialize (mem_is_inv (S n)). cbn in *.
       specialize (mem_is_inv _ _ _ H4 H5).
-      destruct v; eauto.
+      destruct v, d; eauto.
       destruct PRE.
       clear -mem_is_inv st_id_allocated st_id_allocated0 H4 H5.
 
@@ -362,7 +362,7 @@ Proof.
     - unfold no_dshptr_aliasing in *. intros.
       specialize (st_no_dshptr_aliasing (S n) (S n')).
       cbn in st_no_dshptr_aliasing.
-      specialize (st_no_dshptr_aliasing _ _ _ H4 H5).
+      specialize (st_no_dshptr_aliasing _ _ _ _ _ H4 H5).
       inv st_no_dshptr_aliasing. reflexivity.
     - unfold no_llvm_ptr_aliasing_cfg, no_llvm_ptr_aliasing in *.
       intros. cbn* in *.
@@ -377,9 +377,9 @@ Proof.
       intros.
 
       specialize (st_id_allocated (S n)). cbn in *.
-      specialize (st_id_allocated _ _ H4).
+      specialize (st_id_allocated _ _ _ H4).
       clear -st_id_allocated st_id_allocated0 H4.
-      specialize (st_id_allocated0 _ _ _ H4).
+      specialize (st_id_allocated0 _ _ _ _ H4).
       pose proof mem_block_exists_memory_next_key.
 
       rewrite <- mem_block_exists_memory_remove_neq. auto.
