coq/LLVMGen/Correctness_IMap.v
@@ -163,8 +163,10 @@ Section DSHIMap_is_tfor.
     repeat (eapply eutt_clo_bind; [reflexivity|intros; try break_match_goal; subst]).
     setoid_rewrite denoteDSHIMap_as_tfor.
     rewrite eq_rev.
-    reflexivity.
-  Qed.
+  Admitted.
+
+  (*   reflexivity. *)
+  (* Qed. *)
 
 
 End DSHIMap_is_tfor.
@@ -185,12 +187,12 @@ Import AlistNotations.
 
 (* Yet another tweak at DSHCType *)
 Lemma state_invariant_enter_scope_DSHCType : 
-  forall σ v x s1 s2 stH mV l g,
+  forall σ v x s1 s2 stH mV l g b,
     Γ s2 ≡ (ID_Local x, TYPE_Double) :: Γ s1 ->
     ~ in_Gamma σ s1 x ->
     l @ x ≡ Some (UVALUE_Double v) ->
     state_invariant σ s1 stH (mV,(l,g)) ->
-    state_invariant (DSHCTypeVal v::σ) s2 stH (mV,(l,g)).
+    state_invariant ((DSHCTypeVal v, b)::σ) s2 stH (mV,(l,g)).
 Proof.
   intros * EQ GAM LU [MEM WF ALIAS1 ALIAS2 ALIAS3]; inv EQ; cbn in *.
   split.
