coq/LLVMGen/Correctness_MemInit.v
@@ -302,7 +302,7 @@ Proof.
     + Opaque memory_set.
       cbn; intros * LU1 LU2.
       eapply mem_is_inv in LU2; eauto.
-      destruct v; auto.
+      destruct v, d; auto.
       destruct LU2 as (? & ? & ? & ?).
       destruct (n =? a) eqn:EQ.
       * apply beq_nat_true in EQ; subst.
